concurrency/Modular/dataStruct.v
@@ -42,7 +42,7 @@ Proof.
 Defined.
 
 #[export] Instance pointer_lock : Ghost := discrete_PCM (val * val * range).
-Definition ghost_info : Type := (key * val)%type.
+Definition ghost_info : Type := (key * val * (list gname))%type.
 
 (* This allows the range to be outdated while the ghost_info may be present or absent. *)
 #[export] Instance node_ghost : Ghost := prod_PCM pointer_lock (exclusive_PCM (option ghost_info)).
